Change naming convention of permission predicates from is to own and make it clear how to use the send specification for multiple sends.

src/goose_lang/lib/channel/chan_spec_single.v
@@ -127,15 +127,15 @@ From Perennial.Helpers Require Import List ModArith.
  .       
  
  (* Permission to send on the channel *)
- Definition is_UnbufferedChannel_Sender (l: loc) (i: nat) γs: iProp _ :=
+ Definition own_UnbufferedChannel_Sender (l: loc) (i: nat) γs: iProp _ :=
    "HSenderIndex" ∷ ghost_var γs (DfracOwn (1/2)) i
  .
  
- Definition is_UnbufferedChannel_SenderProps (l: loc) (P: iProp Σ) (Q: iProp Σ) (R: iProp Σ) (v: val) (i: nat) (num_uses: nat) (chan_type: ty) γs: iProp _ :=
+ Definition own_UnbufferedChannel_SenderProps (l: loc) (P: iProp Σ) (Q: iProp Σ) (R: iProp Σ) (v: val) (i: nat) (num_uses: nat) (chan_type: ty) γs: iProp _ :=
    ∃ 
    (Ps: list (iProp Σ)) (Qs: list (iProp Σ)) (Vs: list val) γ1 γ2 γ3 γ4 γ5 γr,
    "#HChanHandle" ∷  is_UnbufferedChannel l Ps Qs Vs R num_uses chan_type γs γr γ1 γ2 γ3 γ4 γ5 ∗
-   "HChanHandleSenderPermission" ∷  is_UnbufferedChannel_Sender l i γs ∗
+   "HChanHandleSenderPermission" ∷  own_UnbufferedChannel_Sender l i γs ∗
    (* Make sure we don't have permission when we have sent everything *)
     "%HMax" ∷  ⌜ i < num_uses ⌝  ∗ 
    (* These allow us to specify the props/value that we will 
@@ -152,7 +152,7 @@ From Perennial.Helpers Require Import List ModArith.
  Definition is_UnbufferedChannel_CloserProps (l: loc) (i: nat) (R: iProp Σ) (chan_type: ty) γs: iProp _ :=
    ∃ (Ps: list (iProp Σ)) (Qs: list (iProp Σ)) (Vs: list val) (num_uses: nat) γ1 γ2 γ3 γ4 γ5 γr,
    "Hchanhand" ∷  is_UnbufferedChannel l Ps Qs Vs R num_uses chan_type γs γr γ1 γ2 γ3 γ4 γ5 ∗
-   "Hchanhandsender" ∷  is_UnbufferedChannel_Sender l i γs ∗
+   "Hchanhandsender" ∷  own_UnbufferedChannel_Sender l i γs ∗
    (* Might not be necessary but should make it easier to connect this 
    with the lock invariants *)
    "%HCap" ∷  ⌜ i = num_uses ⌝ ∗ 
@@ -162,23 +162,24 @@ From Perennial.Helpers Require Import List ModArith.
  .
  
  (* If we have sent everything, we can only close. *)
- Definition is_UnbufferedChannel_SenderProps_Or_Closeable
+ Definition own_UnbufferedChannel_SenderProps_Or_Closeable
   (l: loc) (i: nat) (num_uses: nat) (R: iProp Σ) (chan_type: ty) γs: iProp _ :=
  match bool_decide(i < num_uses) with
    | false => is_UnbufferedChannel_CloserProps l i R chan_type γs
-   | true => is_UnbufferedChannel_Sender  l i γs
+   | true => ∃ (P: iProp Σ) (Q: iProp Σ) (v: val),
+   own_UnbufferedChannel_SenderProps  l P Q R v i num_uses chan_type γs
  end
   .
  
- Definition is_UnbufferedChannel_Receiver (l: loc) (i: nat) γr: iProp _ :=
+ Definition own_UnbufferedChannel_Receiver (l: loc) (i: nat) γr: iProp _ :=
    "Hreceiverindex" ∷ ghost_var γr (DfracOwn (1/2)) i
  .
  
- Definition is_UnbufferedChannel_ReceiverProps (l: loc) (P: iProp Σ) (Q: iProp Σ) (R: iProp Σ) (v: val) (i: nat) (num_uses:nat) (chan_type: ty) γr γ5: iProp _ :=
+ Definition own_UnbufferedChannel_ReceiverProps (l: loc) (P: iProp Σ) (Q: iProp Σ) (R: iProp Σ) (v: val) (i: nat) (num_uses:nat) (chan_type: ty) γr γ5: iProp _ :=
    ∃ 
    (Ps: list (iProp Σ)) (Qs: list (iProp Σ)) (Vs: list val)  γ1 γ2 γ3 γ4 γs,
    "#HChanHandle" ∷  is_UnbufferedChannel l Ps Qs Vs R num_uses chan_type γs γr γ1 γ2 γ3 γ4 γ5 ∗
-    "HChanHandleReceiver" ∷  is_UnbufferedChannel_Receiver l i γr ∗
+    "HChanHandleReceiver" ∷  own_UnbufferedChannel_Receiver l i γr ∗
      "%HPsreceiver" ∷  ⌜(nth i Ps True%I) = P⌝ ∗
      "%HQsreceiver" ∷  ⌜ (nth i Qs True%I) = Q ⌝ ∗
      "%Hvsreceiver" ∷ ⌜ (nth i Vs (zero_val chan_type)) = v ⌝ ∗ 
@@ -192,7 +193,7 @@ From Perennial.Helpers Require Import List ModArith.
  Once we know a channel is able to be closed, we know the sender 
  won't send anything else and receive on a closed channel always returns the
  same thing. *)
- Definition is_UnbufferedChannel_ReceiverClosed (l: loc) (i: nat) (R: iProp Σ) γr γ5: iProp _ :=
+ Definition own_UnbufferedChannel_ReceiverClosed (l: loc) (i: nat) (R: iProp Σ) γr γ5: iProp _ :=
    ∃ (Ps: list (iProp Σ)) (Qs: list (iProp Σ)) (Vs: list val) (num_uses: nat) (chan_type:ty) γ1 γ2 γ3 γ4 γs,
    "#Hchanhand" ∷  is_UnbufferedChannel l Ps Qs Vs R num_uses chan_type γs γr γ1 γ2 γ3 γ4 γ5 ∗
    "%HCap" ∷  ⌜ i = num_uses ⌝ ∗ 
@@ -206,33 +207,33 @@ From Perennial.Helpers Require Import List ModArith.
  so that other threads can pointlessly receive on a closed channel and 
  return the null value. I am trying to be minimal here since it may be 
  possible in the future to regain the original permissions *)
- Definition is_UnbufferedChannel_ReceiverConsumeCloseProp (l: loc) (i: nat) (R: iProp Σ) γr γ5: iProp _ :=
-   "#HRecClosed" ∷ is_UnbufferedChannel_ReceiverClosed l i R γr γ5 ∗ 
+ Definition own_UnbufferedChannel_ReceiverConsumeCloseProp (l: loc) (i: nat) (R: iProp Σ) γr γ5: iProp _ :=
+   "#HRecClosed" ∷ own_UnbufferedChannel_ReceiverClosed l i R γr γ5 ∗ 
    "HReceiverClosedProp" ∷  ghost_var γ5 (DfracOwn (1/2)) true   
  .
  
  (* Once we have received all of the values we know the sender will not send
  anymore but may close the channel. Note that we can regain 
- is_UnbufferedChannel_Receiver from the persistent props so we only need to retain
+ own_UnbufferedChannel_Receiver from the persistent props so we only need to retain
  the receiver permission to receive again. *)
- Definition is_UnbufferedChannel_ReceiverProps_Or_Closed
+ Definition own_UnbufferedChannel_ReceiverProps_Or_Closed
   (l: loc) (i: nat) (num_uses: nat) (R: iProp Σ) (chan_type: ty) γr γ5: iProp _ :=
  match bool_decide(i < num_uses) with
-   | false =>  is_UnbufferedChannel_ReceiverConsumeCloseProp l i R γr γ5
+   | false =>  own_UnbufferedChannel_ReceiverConsumeCloseProp l i R γr γ5
    | true => 
    (∃ (P: iProp Σ) (Q: iProp Σ) (v: val),
-   is_UnbufferedChannel_ReceiverProps l P Q R v i num_uses chan_type γr γ5)
+   own_UnbufferedChannel_ReceiverProps l P Q R v i num_uses chan_type γr γ5)
  end
   .
  
  Definition TryReceive_Success (l: loc) 
  (P: iProp Σ) (R: iProp Σ) (v: val) (i: nat) (num_uses: nat) (chan_type: ty) γr γ5 : iProp _ :=
- is_UnbufferedChannel_ReceiverProps_Or_Closed
+ own_UnbufferedChannel_ReceiverProps_Or_Closed
      l (i + 1) num_uses R chan_type γr γ5 ∗ P.
  
  Definition TryReceive_SenderNotReady (l: loc) 
  (P: iProp Σ)  (Q: iProp Σ) (R: iProp Σ) (v: val) (i: nat) (num_uses: nat) (chan_type: ty) γr γ5 : iProp _ :=
-  is_UnbufferedChannel_ReceiverProps l P Q R v i num_uses chan_type γr γ5 ∗ Q.
+  own_UnbufferedChannel_ReceiverProps l P Q R v i num_uses chan_type γr γ5 ∗ Q.
  
  Definition TryReceive_Xor (l: loc) 
  (P: iProp Σ) (Q: iProp Σ) (R: iProp Σ) (v: val) (i: nat) (num_uses: nat) (chan_type: ty) γr γ5 ret_bool ret_val : iProp _ :=
@@ -256,13 +257,13 @@ From Perennial.Helpers Require Import List ModArith.
    {{{ True }}}
      NewChannel chan_type #()
    {{{(l: loc) γs γr γ1 γ2 γ3 γ4 γ5, RET #l; 
-   is_UnbufferedChannel_ReceiverProps l (hd True%I Ps) (hd True%I Qs) R (hd (zero_val chan_type) Vs) 0 num_uses chan_type γr γ5 ∗
-   is_UnbufferedChannel_SenderProps l (hd True%I Ps) (hd True%I Qs) R (hd (zero_val chan_type) Vs) 0 num_uses chan_type γs  ∗
+   own_UnbufferedChannel_ReceiverProps l (hd True%I Ps) (hd True%I Qs) R (hd (zero_val chan_type) Vs) 0 num_uses chan_type γr γ5 ∗
+   own_UnbufferedChannel_SenderProps l (hd True%I Ps) (hd True%I Qs) R (hd (zero_val chan_type) Vs) 0 num_uses chan_type γs  ∗
     is_UnbufferedChannel l Ps Qs Vs R num_uses chan_type γs γr γ1 γ2 γ3 γ4 γ5
     }}}.
  Proof.
  Admitted. 
- 
+
  (* By proving P and sending v, we can gain Q. i is the number of times we 
  have sent so far which is used as an index into the lists of propositions
   and values that we declare when we initialize the channel.
@@ -272,10 +273,10 @@ From Perennial.Helpers Require Import List ModArith.
  (P: iProp Σ) (Q: iProp Σ) (R: iProp Σ) (v: val) (i: nat) (num_uses: nat) (chan_type: ty) γs :
  val_ty v chan_type -> 
  i + 1 < 2 ^ 63 ->
-   {{{ is_UnbufferedChannel_SenderProps l P Q R v i num_uses chan_type γs ∗ P }}}
+   {{{ own_UnbufferedChannel_SenderProps l P Q R v i num_uses chan_type γs ∗ P }}}
     Channel__Send chan_type #l v
    {{{ RET #(); 
-   is_UnbufferedChannel_SenderProps_Or_Closeable l (i + 1) num_uses R chan_type γs ∗ Q  }}}.
+   own_UnbufferedChannel_SenderProps_Or_Closeable l (i + 1) num_uses R chan_type γs ∗ Q  }}}.
  Proof.
    Admitted.
  
@@ -284,9 +285,9 @@ From Perennial.Helpers Require Import List ModArith.
  into the lists of propositions and values. *)
  Lemma wp_ReusableChanHandle__Receive (l: loc) 
  (P: iProp Σ) (Q: iProp Σ) (R: iProp Σ) (v: val) (i: nat) (num_uses: nat) (chan_type: ty) γr γ5 :
-   {{{ is_UnbufferedChannel_ReceiverProps l P Q R v i num_uses chan_type γr γ5 ∗ Q }}}
+   {{{ own_UnbufferedChannel_ReceiverProps l P Q R v i num_uses chan_type γr γ5 ∗ Q }}}
      Channel__Receive chan_type #l
-   {{{ RET (v, #false); is_UnbufferedChannel_ReceiverProps_Or_Closed
+   {{{ RET (v, #false); own_UnbufferedChannel_ReceiverProps_Or_Closed
      l (i + 1) num_uses R chan_type γr γ5 ∗ P }}}.
  Proof.
    Admitted.
@@ -298,9 +299,9 @@ From Perennial.Helpers Require Import List ModArith.
  proposition R which can only be gained once. *)
  Lemma wp_ReusableChanHandle__ReceiveConsumeCloseProp 
   (l: loc) (R: iProp Σ) (i: nat) (chan_type: ty) γr γ5:
-  {{{ is_UnbufferedChannel_ReceiverConsumeCloseProp l i R γr γ5 }}}
+  {{{ own_UnbufferedChannel_ReceiverConsumeCloseProp l i R γr γ5 }}}
      Channel__Receive chan_type #l
-   {{{ RET ( (zero_val chan_type), #true); is_UnbufferedChannel_ReceiverClosed l i R γr γ5 ∗ R }}}.
+   {{{ RET ( (zero_val chan_type), #true); own_UnbufferedChannel_ReceiverClosed l i R γr γ5 ∗ R }}}.
  Proof.
    Admitted. 
  
@@ -312,7 +313,7 @@ From Perennial.Helpers Require Import List ModArith.
  use TryReceive in Goose.  *)
  Lemma wp_UnbufferedChannel__ReceiveClosed 
   (l: loc) (R: iProp Σ) (i: nat) (chan_type: ty) γr γ5:
-  {{{  is_UnbufferedChannel_ReceiverClosed l i R γr γ5  }}}
+  {{{  own_UnbufferedChannel_ReceiverClosed l i R γr γ5  }}}
      Channel__Receive chan_type #l
    {{{ RET ( (zero_val chan_type), #true); True }}}.
  Proof.
@@ -331,7 +332,7 @@ From Perennial.Helpers Require Import List ModArith.
  
  Lemma wp_ReusableChanHandle__TryReceive (l: loc) 
  (P: iProp Σ) (Q: iProp Σ) (R: iProp Σ) (v: val) (i: nat) (num_uses: nat) (chan_type: ty) γr γ5 :
-   {{{ is_UnbufferedChannel_ReceiverProps l P Q R v i num_uses chan_type γr γ5 ∗ Q }}}
+   {{{ own_UnbufferedChannel_ReceiverProps l P Q R v i num_uses chan_type γr γ5 ∗ Q }}}
      Channel__TryReceive chan_type #l
    {{{ (ret_bool: bool) (ret_val: val),  
      RET (#ret_bool, ret_val, #false); 
@@ -342,11 +343,11 @@ From Perennial.Helpers Require Import List ModArith.
  
  Definition TryReceiveClosedPropConsume_Success (l: loc) 
  (R: iProp Σ) (i: nat) γr γ5 : iProp _ :=
- is_UnbufferedChannel_ReceiverClosed l i R γr γ5 ∗ R.
+ own_UnbufferedChannel_ReceiverClosed l i R γr γ5 ∗ R.
  
  Definition TryReceive_CloserNotReady (l: loc) 
   (R: iProp Σ) (i: nat) γr γ5 : iProp _ :=
-  is_UnbufferedChannel_ReceiverConsumeCloseProp l i R γr γ5.
+  own_UnbufferedChannel_ReceiverConsumeCloseProp l i R γr γ5.
  
  Definition TryReceiveClosedPropConsume_Xor (l: loc) 
  (R: iProp Σ) (i: nat) γr γ5 ret_bool : iProp _ :=
@@ -365,7 +366,7 @@ From Perennial.Helpers Require Import List ModArith.
  return false. *)
  Lemma wp_ReusableChanHandle__TryReceiveClosed 
   (l: loc) (R: iProp Σ) (i: nat) (chan_type: ty) γr γ5:
-  {{{ is_UnbufferedChannel_ReceiverConsumeCloseProp l i R γr γ5 }}}
+  {{{ own_UnbufferedChannel_ReceiverConsumeCloseProp l i R γr γ5 }}}
      Channel__TryReceive chan_type #l
    {{{ (ret_bool: bool),  RET ( #ret_bool ,(zero_val chan_type),  #ret_bool);
     TryReceiveClosedPropConsume_Xor l R i γr γ5 ret_bool }}}.
@@ -374,11 +375,11 @@ From Perennial.Helpers Require Import List ModArith.
  
  Definition TrySend_Success (l: loc) 
  (Q: iProp Σ) (R: iProp Σ) (v: val) (i: nat) (num_uses: nat) (chan_type: ty) γs : iProp _ :=
- is_UnbufferedChannel_SenderProps_Or_Closeable l (i + 1) num_uses R chan_type γs ∗ Q.
+ own_UnbufferedChannel_SenderProps_Or_Closeable l (i + 1) num_uses R chan_type γs ∗ Q.
  
  Definition TrySend_Failure (l: loc) 
  (P: iProp Σ)  (Q: iProp Σ) (R: iProp Σ) (v: val) (i: nat) (num_uses: nat) (chan_type: ty) γs : iProp _ :=
-   is_UnbufferedChannel_SenderProps l P Q R v i num_uses chan_type γs ∗ P.
+   own_UnbufferedChannel_SenderProps l P Q R v i num_uses chan_type γs ∗ P.
  
  Definition TrySend_Xor (l: loc) 
  (P: iProp Σ) (Q: iProp Σ) (R: iProp Σ) (v: val) (i: nat) (num_uses: nat) chan_type γs ret_val : iProp _ :=
@@ -394,7 +395,7 @@ From Perennial.Helpers Require Import List ModArith.
  (P: iProp Σ) (Q: iProp Σ) (R: iProp Σ) (v: val) (i: nat) (num_uses: nat) (chan_type: ty) γs :
  val_ty v chan_type -> 
  i + 1 < 2 ^ 63 ->
-   {{{ is_UnbufferedChannel_SenderProps l P Q R v i num_uses chan_type γs ∗ P }}}
+   {{{ own_UnbufferedChannel_SenderProps l P Q R v i num_uses chan_type γs ∗ P }}}
     Channel__TrySend chan_type #l v
    {{{ (ret_val: bool), RET #ret_val;
    TrySend_Xor l P Q R v i num_uses chan_type γs ret_val }}}.
